fairness/lawyer/eo_fin.v
@@ -1,0 +1,45 @@
+From iris.proofmode Require Import tactics coq_tactics.
+(* From iris.algebra Require Import auth gmap gset excl. *)
+(* From iris.base_logic Require Export gen_heap. *)
+(* From trillium.program_logic Require Export weakestpre adequacy ectx_lifting. *)
+From trillium.fairness Require Import locales_helpers utils.
+From trillium.fairness.lawyer Require Import obligations_model obls_utils obligations_resources program_logic.
+From trillium.fairness.heap_lang Require Export heap_lang_defs tactics notation sswp_logic locales_helpers_hl.
+
+
+Close Scope Z.
+
+(* Definition EODegree n := Fin.t (S n). *)
+(* Definition EOLevel n := Fin.t (S n). *)
+Definition EODegree n := { i | i < n }. 
+Definition EOLevel n := { i | i < n }. 
+
+Section EoFin.
+  Context (LIM: nat).
+  Let MAX_OBL_STEPS := 10.
+  
+  Instance EO_OP: ObligationsParams (EODegree LIM) (EOLevel LIM) (locale heap_lang) MAX_OBL_STEPS.
+  Proof using.
+    esplit; try by apply _.
+    - rewrite /EODegree.
+      exact (fun d1 d2 => proj1_sig d1 < proj1_sig d2).
+    - exact (fun d1 d2 => proj1_sig d1 < proj1_sig d2).
+  Defined.
+
+  Let OM := ObligationsModel EO_OP.
+
+  Let EODegreeOfe := sigO (fun i => i < LIM). 
+  Let EOLevelOfe := sigO (fun i => i < LIM).
+
+  Instance foo: LeibnizEquiv EOLevelOfe.
+  Admitted. 
+  
+  Let EM := @ObligationsEM EODegreeOfe EOLevelOfe _ _ _ heap_lang _ _ _ EO_OP. 
+
+  Context `{hGS: @heapGS Σ _ EM}.
+  Let oGS : ObligationsGS EO_OP Σ := heap_fairnessGS (heapGS := hGS).
+
+  
+
+
+End EoFin.
